AttarchTrans.v
@@ -1,0 +1,83 @@
+Require Import Ctl.Definition.
+Require Import TransitionSystems.
+Require Import SepLogic.
+
+(* Maybe sel4 should not be its own place *)
+Inductive component : Set := 
+  | sel4 
+  | platam 
+  | vmm 
+  | useram.
+
+Inductive loc : Set :=
+  | boot_ev 
+  | vm_ev
+  | useram_key.
+
+(* Add linux state under vm? *)
+(* Note, all sudoers have access to useram/platam channel *)
+Inductive useram_state : Set :=
+  | useram_waiting_key (* initial state *)
+  | useram_waiting_request
+  | useram_measuring
+  | useram_making_request
+  | useram_sending_response.
+
+Inductive useram_trans : transition (sprop component loc) useram_state :=
+  | useram_get_key : forall (acc: access component) (k: nat),
+      acc useram read ->
+      useram_trans
+          (acc @ useram_key ** useram_key ↦ k, useram_waiting_key)
+          (acc @ useram_key ** useram_key ↦ k, useram_waiting_request)
+  (* | useram_get_request : useram_trans 
+      (s, useram_waiting_key)
+      (s,useram_) *)
+  .
+(* Definition useram_strans := stransition useram_trans. *)
+
+Inductive platam_state : Set :=
+  | platam_init
+  | platam_appraise
+  | platam_run.
+
+Definition good_vm_ev : nat. Admitted.
+Definition bad_vm_ev  : nat. Admitted.
+Inductive platam_trans : transition (sprop component loc) platam_state :=
+  | platam_measure_good_vm : platam_trans
+      (empty, platam_init)
+      (private platam @ vm_ev ** vm_ev ↦ good_vm_ev, platam_appraise)
+  | platam_measure_bad_vm : platam_trans
+      (empty, platam_init)
+      (private platam @ vm_ev ** vm_ev ↦ bad_vm_ev, platam_appraise)
+  | platam_appraise_good_vm : forall (acc: access component),
+      acc platam read ->
+      platam_trans
+          (acc @ vm_ev ** vm_ev ↦ good_vm_ev, platam_appraise)
+          (acc @ vm_ev ** vm_ev ↦ good_vm_ev, platam_run).
+
+Inductive vm_state : Set :=
+  | vm_init
+  | vm_run : useram_state -> vm_state.
+
+Definition vm_trans : transition (sprop component loc) vm_state. Admitted.
+
+Inductive attarch_state : Set :=
+  | boot_from_good_plat (* initial state *)
+  | boot_from_bad_plat  (* initial state *)
+  | sel4_run : platam_state * vm_state -> attarch_state.
+
+Definition good_boot_ev : nat. Admitted.
+Definition bad_boot_ev  : nat. Admitted.
+Inductive attarch_trans : transition (sprop component loc) attarch_state :=
+  | good_boot : attarch_trans 
+      (empty, boot_from_good_plat)
+      ((acc_at boot_ev readonly) ** boot_ev ↦ good_boot_ev, sel4_run (platam_init, vm_init))
+  | bad_boot : attarch_trans 
+      (empty, boot_from_bad_plat)
+      (acc_at boot_ev readonly ** boot_ev ↦ bad_boot_ev, sel4_run (platam_init, vm_init))
+  | component_step : forall g g' s s',
+      (platam_trans ⊔ vm_trans) (g,s) (g',s') ->
+      attarch_trans 
+          (g, sel4_run s)
+          (g', sel4_run s').
+Definition attarch_strans := stransition attarch_trans.
