BinaryRelations.v
@@ -1,0 +1,21 @@
+Require Import Coq.Relations.Relation_Definitions.
+Require Import Coq.Relations.Relation_Operators.
+
+Require Import Coq.Lists.List.
+
+Definition rel_singleton {A} (x y : A): relation A :=
+  fun x' y' => x' = x /\ y' = y -> True.
+
+(* Notation for reflexive transitive closures *)
+Notation "R ^*" := (clos_refl_trans _ R) (at level 35).
+
+Definition is_serial {A} (R: relation A) := forall a, exists b, R a b.
+Definition serial A := {R: relation A | is_serial R}.
+
+Definition reachable {A} (R: relation A) (l: list A) (b: A) := exists a, In a l /\ R^* a b.
+
+Inductive steps : nat -> forall {A}, relation A -> relation A :=
+  | steps_one   : forall {A} (R: relation A) x y,
+      R x y -> steps 1 R x y
+  | steps_multi : forall {A} n (R: relation A) x y z,
+      steps n R x y -> R y x -> steps (S n) R x z.
