SepLogic.v
@@ -1,0 +1,46 @@
+Notation component := nat (only parsing).
+
+Inductive privilege : Set :=
+  | read 
+  | write 
+  | exec.
+
+Definition access component := component -> privilege -> Prop.
+Inductive readonly {component} : access component :=
+  | ro : forall c, readonly c read.
+
+Inductive private {component} (c: component): access component :=
+  | anyPriv : forall (p: privilege), private c c p.
+
+(* Is acc_at a spatial predicate? I think so *)
+Inductive sprop (comp loc: Set) :=
+  | sep_con : sprop comp loc -> sprop comp loc -> sprop comp loc
+  (* | sep_at  : forall v, loc -> access -> v -> sprop loc *)
+  | val_at  : forall v, loc -> v -> sprop comp loc
+  | acc_at  : loc -> access comp -> sprop comp loc
+  | empty   : sprop comp loc.
+
+Arguments sep_con {comp loc}%type_scope.
+Arguments val_at  {comp loc v}%type_scope.
+Arguments acc_at  {comp loc}%type_scope.
+Arguments empty   {comp loc}%type_scope.
+
+(* Declare Scope sep_scope. *)
+(* Bind Scope sep_scope with sprop. *)
+
+(* Not sure why this is disallowed. Todo, look at other coq sep logics. *)
+(* Notation "X * Y" := (sep_con X Y) (at level 45, right associativity) : sep_scope. *)
+Notation "X ** Y" := (sep_con X Y) (at level 55, right associativity).
+Notation "l ↦ v" := (val_at l v) (at level 50).
+(* Also not sure why this one isn't working *)
+(* Notation "l : V ↦ v" := (@val_at _ _ V l v) (at level 40). *)
+(* Check (0 ↦ 1). *)
+(* Check (0 : nat ↦ 1). *)
+Notation "a @ l" := (acc_at l a) (at level 50).
+
+Reserved Notation "X ⊢ Y" (at level 70).
+(* Reserved Notation "X ⊬ Y" (at level 70). *)
+Inductive sEntails {comp loc} : sprop comp loc -> sprop comp loc -> Prop :=
+  | sep_con_comm  : forall X Y, X ** Y ⊢ Y ** X
+  | sep_con_assoc : forall X Y Z, X ** Y ** Z ⊢ (X ** Y) ** Z
+  where "X ⊢ Y" := (sEntails X Y).
