TransitionSystems.v
@@ -1,0 +1,58 @@
+Require Import Coq.Relations.Relation_Definitions.
+Require Import SepLogic.
+
+(* Definition transition A := relation (A * sprop nat). *)
+(* A is global state, B is local *)
+Definition transition A B := relation (A * B).
+
+(* This is effectively a union *)
+(* This mirrors Chlipala's definition of concurrent transitions in FRAP *)
+(* Can nested transitions have "globals" for various levels? *)
+(* Inductive either_transition {A B} (R: transition A) (Q: transition B) : transition (A * B) :=
+  | step_l : forall a a' b s s',
+      R (a,s) (a',s') -> either_transition R Q ((a,b),s) ((a',b),s')
+  | step_r : forall a b b' s s',
+      Q (b,s) (b',s') -> either_transition R Q ((a,b),s) ((a,b'),s'). *)
+Inductive either_transition {G A B} (R: transition G A) (Q: transition G B) : transition G (A * B) :=
+  | step_l : forall g g' a a' b,
+      R (g,a) (g',a') -> either_transition R Q (g,(a,b)) (g',(a',b))
+  | step_r : forall g g' a b b',
+      Q (g,b) (g',b') -> either_transition R Q (g,(a,b)) (g',(a,b')).
+    
+(* Definition sprop_union {loc} : sprop loc -> sprop loc -> sprop loc. Admitted. *)
+(* Is this a useful abstraction, distinct from either? *)
+(* Inductive concurrent_transitions {G A B} (gunion : G -> G -> G) (R: transition G A) (Q: transition G B) : transition G (A * B) :=
+  | step_lr   : forall s s', either_transition R Q s s' -> concurrent_transitions gunion R Q s s'
+  | step_both : forall g g' g'' a a' b b',
+      R (g,a) (g,a') -> 
+      Q (g,b) (g,b') -> 
+      concurrent_transitions gunion R Q (g,(a,b)) (gunion g' g'', (a',b')). *)
+      
+Notation "R ⊔ S" := (either_transition R S) (at level 70).
+(* Notation "R ∥ S" := (concurrent_transitions R S) (at level 70). *)
+
+(* TODO: non-starving variation. *)
+(* Uses the fuel idiom? *)
+(* n is the number of steps it can take in a row in one transition *)
+(* Inductive either_transition_nostarve {A B} (R: transition A) (Q: transition B) (n m r: nat) : transition (A * B) :=
+  | steps_l : forall a a' b s s',
+      R (a,s) (a',s') -> either_transition_nostarve R Q n n r ((a,b),s) ((a',b),s')
+  | steps_r : forall a b b' s s',
+      Q (b,s) (b',s') -> either_transition_nostarve R Q ((a,b),s) ((a,b'),s').
+ 
+Notation "R ⊕ S" := (either_transition_nostarve R S) (at level 70). *)
+
+(* Todo, support hoare logic syntax of relations? *)
+Inductive stransition {comp loc A} (R: transition (sprop comp loc) A) : transition (sprop comp loc) A :=
+  | frame_rule : forall Q Q' S a a',
+      R (Q,a) (Q',a') ->
+      (* Nothing "modified" by R free in S? -> *)
+      stransition R (Q ** S, a) (Q' ** S, a')
+  | sentails_pre : forall Q Q' S a a',
+      Q ⊢ S ->
+      stransition R (Q,a) (Q',a') ->
+      stransition R (S,a) (Q',a')
+  | sentails_post : forall Q Q' S a a',
+      Q' ⊢ S ->
+      stransition R (Q,a) (Q',a') ->
+      stransition R (Q,a) (S,a').
